Use Equations everywhere in Checker as well

template-coq/theories/Induction.v
@@ -1,6 +1,6 @@
 (* Distributed under the terms of the MIT license.   *)
 
-From MetaCoq Require Import BasicAst Ast AstUtils.
+From MetaCoq Require Import utils BasicAst Ast AstUtils.
 Require Import List Program.
 Require Import BinPos.
 Require Import Coq.Arith.Compare_dec Bool.
@@ -40,7 +40,7 @@ Lemma term_forall_list_ind :
 Proof.
   intros until t. revert t.
   fix auxt 1.
-  move auxt at top. 
+  move auxt at top.
   destruct t;
     match goal with
       H : _ |- _ => apply H; auto
@@ -135,3 +135,47 @@ Proof.
   induction H16. constructor.
   inv H18; constructor; intuition auto.
 Qed.
+
+Definition tCaseBrsType {A} (P : A -> Type) (l : list (nat * A)) :=
+  All (fun x => P (snd x)) l.
+
+Definition tFixType {A : Set} (P P' : A -> Type) (m : mfixpoint A) :=
+  All (fun x : def A => P x.(dtype) * P' x.(dbody))%type m.
+
+Lemma term_forall_list_rect :
+  forall P : term -> Type,
+    (forall n : nat, P (tRel n)) ->
+    (forall i : ident, P (tVar i)) ->
+    (forall (n : nat) (l : list term), All P l -> P (tEvar n l)) ->
+    (forall s, P (tSort s)) ->
+    (forall t : term, P t -> forall (c : cast_kind) (t0 : term), P t0 -> P (tCast t c t0)) ->
+    (forall (n : name) (t : term), P t -> forall t0 : term, P t0 -> P (tProd n t t0)) ->
+    (forall (n : name) (t : term), P t -> forall t0 : term, P t0 -> P (tLambda n t t0)) ->
+    (forall (n : name) (t : term),
+        P t -> forall t0 : term, P t0 -> forall t1 : term, P t1 -> P (tLetIn n t t0 t1)) ->
+    (forall t : term, P t -> forall l : list term, All P l -> P (tApp t l)) ->
+    (forall (s : String.string) (u : list Level.t), P (tConst s u)) ->
+    (forall (i : inductive) (u : list Level.t), P (tInd i u)) ->
+    (forall (i : inductive) (n : nat) (u : list Level.t), P (tConstruct i n u)) ->
+    (forall (p : inductive * nat) (t : term),
+        P t -> forall t0 : term, P t0 -> forall l : list (nat * term),
+            tCaseBrsType P l -> P (tCase p t t0 l)) ->
+    (forall (s : projection) (t : term), P t -> P (tProj s t)) ->
+    (forall (m : mfixpoint term) (n : nat), tFixType P P m -> P (tFix m n)) ->
+    (forall (m : mfixpoint term) (n : nat), tFixType P P m -> P (tCoFix m n)) ->
+    forall t : term, P t.
+Proof.
+  intros until t. revert t.
+  fix auxt 1.
+  move auxt at top.
+  destruct t;
+    match goal with
+      H : _ |- _ => apply H; auto
+    end;
+    match goal with
+      |- _ P ?arg =>
+      revert arg; fix aux_arg 1; intro arg;
+        destruct arg; constructor; [|apply aux_arg];
+          try split; apply auxt
+    end.
+Defined.
